\documentclass[UTF8]{ctexart}
\usepackage{amsmath,amssymb,amsfonts}
\usepackage{graphicx}%插入图片的宏包。
\usepackage{tikz}%画图功能宏包
\title{CMP模型公式}
\author{向涛:湘潭大学}
\date{\today}
\usepackage{geometry}
\geometry{left=2cm,right=2cm,top=2cm,bottom=2cm}
\begin{document}
\maketitle

\section{不加磁场的公式}

\begin{equation}
\left \{
\begin{aligned}
& \overline{G}=G_h \cup \Gamma_h=\{ (x_j,t_k):0\leq j\leq N;0\leq k \leq M \}　\\
& G_h = \{ (x_j,t_k):0<j<N;0<k\leq M \} \\
& \Gamma_h=\{ (x_j,t_k):j=0,N;k=1,\cdots,M \} \cup \{  (x_j,t_0):j=0,\cdots,N \}
\end{aligned}
\right.
\end{equation}

\begin{equation}
\nabla\cdot\pmb{u} = 0
\end{equation}

\begin{equation}
\dfrac{\partial u_1}{\partial x} 
+ \dfrac{\partial u_2}{\partial y} 
+ \dfrac{\partial u_3}{\partial z}=0
\end{equation}

\begin{equation}
\rho\dfrac{\partial \pmb{u}}{\partial t}
+ \rho\pmb{u}\cdot\nabla \pmb{u}
= -\nabla p+ \eta\Delta \pmb{u} +\rho\pmb{F}
\end{equation}

\begin{equation}
\left \{
\begin{aligned}
\rho \left(\dfrac{\partial u_1}{\partial t}
+u_1 \dfrac{\partial u_1}{\partial x}
+u_2 \dfrac{\partial u_1}{\partial y}
+u_3 \dfrac{\partial u_1}{\partial z}\right)
= -\dfrac{\partial p}{\partial x} + \eta
\left( \dfrac{\partial^2 u_1}{\partial x^2} + \dfrac{\partial^2 u_1}{\partial y^2}
+\dfrac{\partial^2 u_1}{\partial z^2}  \right) \\
\rho \left(\dfrac{\partial u_2}{\partial t}
+u_1 \dfrac{\partial u_2}{\partial x}
+u_2 \dfrac{\partial u_2}{\partial y}
+u_3 \dfrac{\partial u_2}{\partial z}\right)
= -\dfrac{\partial p}{\partial y} + \eta
\left( \dfrac{\partial^2 u_2}{\partial x^2} + \dfrac{\partial^2 u_2}{\partial y^2}
+\dfrac{\partial^2 u_2}{\partial z^2}  \right)\\
\rho \left(\dfrac{\partial u_3}{\partial t}
+u_1 \dfrac{\partial u_3}{\partial x}
+u_2 \dfrac{\partial u_3}{\partial y}
+u_3 \dfrac{\partial u_3}{\partial z}\right)
= -\dfrac{\partial p}{\partial z} + \eta
\left( \dfrac{\partial^2 u_3}{\partial x^2} + \dfrac{\partial^2 u_3}{\partial y^2}
+\dfrac{\partial^2 u_3}{\partial z^2}  \right)
\end{aligned}
\right.
\end{equation}

\begin{equation}
\left \{
\begin{aligned}
\dfrac{\partial p}{\partial x}
+\rho u_1 \dfrac{\partial u_1}{\partial x}
+\rho u_2 \dfrac{\partial u_1}{\partial y}
&= \eta \dfrac{\partial^2 u_1}{\partial z^2} \\
\dfrac{\partial p}{\partial y}
+\rho u_1 \dfrac{\partial u_2}{\partial x}
+\rho u_2 \dfrac{\partial u_2}{\partial y}
&= \eta \dfrac{\partial^2 u_2}{\partial z^2}
\\
 \dfrac{\partial p}{\partial z} &= 0
\end{aligned}
\right.
\end{equation}

\begin{equation}
\left \{
\begin{aligned}
x=r\cos\theta \\
y=r\sin\theta \\
z=z
\end{aligned}
\right.
\end{equation}

\begin{equation}
\left \{
\begin{aligned}
\dfrac{\partial x}{\partial r} = \cos\theta
~~~ \dfrac{\partial x}{\partial \theta}
= -r\cdot \sin\theta \\
\dfrac{\partial y}{\partial r} = \cos\theta
~~~ \dfrac{\partial y}{\partial \theta}
= r\cdot \cos\theta
\end{aligned}
\right.
\end{equation}

\begin{equation}
\left \{
\begin{aligned}
\dfrac{\partial r}{\partial x} = \cos\theta
~~~ \dfrac{\partial \theta}{\partial x}
= -\dfrac{\sin\theta}{r} \\
\dfrac{\partial r}{\partial y} = \cos\theta
~~~ \dfrac{\partial \theta}{\partial y}
= \dfrac{\cos\theta}{r} 
\end{aligned}
\right.
\end{equation}

\begin{equation}
\left \{
\begin{aligned}
u_1 &= \omega\cdot\cos\theta-u\cdot\sin\theta \\
u_2 &= \omega\cdot\sin\theta+u\cdot\cos\theta 
\end{aligned}
\right.
\end{equation}



\section{加磁场后}








\end{document}